feature(Sepref_Basic) define hn_refine

thys/sepref/Sepref_Basic.thy
@@ -3,13 +3,15 @@ theory Sepref_Basic
 imports 
   "../ds/LLVM_DS_NArray"
   "HOL-Eisbach.Eisbach"
-  Refine_Monadic_Add
+  (* Refine_Monadic_Add *)
   "Lib/Sepref_Misc"
   "Lib/Structured_Apply"
   Sepref_Id_Op
+  "../nrest/NREST"
 begin
+(*
 no_notation i_ANNOT (infixr ":::\<^sub>i" 10)
-no_notation CONST_INTF (infixr "::\<^sub>i" 10)
+no_notation CONST_INTF (infixr "::\<^sub>i" 10) *)
 
 no_notation pred_K ("\<langle>_\<rangle>")
 
@@ -172,14 +174,61 @@ text {* Predicate that expresses refinement. Given a heap
   a concrete result that is related with predicate @{text "R"} to some
   abstract result from @{text "m"}*}
   
-definition "hn_refine \<Gamma> c \<Gamma>' R m \<equiv> nofail m \<longrightarrow>
-  llvm_htriple \<Gamma> c (\<lambda>r. \<Gamma>' ** (EXS x. R x r ** \<up>(RETURN x \<le> m)))"
+definition "hn_refine' \<Gamma> c \<Gamma>' R m \<equiv> nofailT m \<longrightarrow>
+  llvm_htriple \<Gamma> c (\<lambda>r. \<Gamma>' ** (EXS x. R x r ** \<up>(RETURNT x \<le> m)))"
 
-lemma hn_refineI[intro?]:
-  assumes "nofail m 
-    \<Longrightarrow> llvm_htriple \<Gamma> c (\<lambda>r. \<Gamma>' ** (EXS x. R x r ** \<up>(RETURN x \<le> m)))"
-  shows "hn_refine \<Gamma> c \<Gamma>' R m"
-  using assms unfolding hn_refine_def by blast
+
+thm hn_refine'_def[unfolded htriple_def wp_alt ll_\<alpha>_def lift_\<alpha>_cost_def, no_vars, simplified]
+thm wp_alt
+
+definition "hn_refine \<Gamma> c \<Gamma>' R m \<equiv>
+  nofailT m \<longrightarrow>
+  (\<forall>F s cr M. m = REST M \<longrightarrow>
+      llSTATE (\<Gamma> \<and>* F) (s,cr) \<longrightarrow> 
+      (\<exists>ra Ca. M ra \<ge> Some Ca
+        \<longrightarrow> wp c (\<lambda>r. llSTATE (\<Gamma>' \<and>* R ra r \<and>* F \<and>* GC)) (s, cr+Ca)
+      )
+  )"
+
+
+ 
+experiment
+begin
+
+thm htriple_vcgI[no_vars]
+
+lemma hnr_vcgI[htriple_vcg_intros]: 
+  assumes "\<And>F s cr M. \<lbrakk> m = REST M; llSTATE (\<Gamma>**F) (s,cr) \<rbrakk>
+          \<Longrightarrow> (\<exists>ra Ca. M ra \<ge> Some Ca \<longrightarrow>
+                     EXTRACT (wp c (\<lambda>r. POSTCOND ll_\<alpha> (\<Gamma>' ** R ra r ** F ** GC)) (s,cr+Ca)))"
+  shows "hn_refine \<Gamma> c \<Gamma>' R m"  
+  using assms by (simp add: hn_refine_def vcg_tag_defs) 
+
+
+(* TODO: Move *)
+
+lemma "RETURNT x = SPECT M \<longleftrightarrow> M = [x\<mapsto>0]"
+  by(auto simp: RETURNT_def)
+
+lemma ecost_le_zero: "(Ca::ecost) \<le> 0 \<longleftrightarrow> Ca=0"
+  apply(cases Ca) by(auto simp: zero_acost_def less_eq_acost_def)
+
+
+lemma hnr_RETURN_pass:
+  "hn_refine (hn_ctxt R x p) (return p) (hn_invalid R x p) R (RETURNT x)"
+  \<comment> \<open>Pass on a value from the heap as return value\<close>
+  apply (subst invalidate_clone')
+  unfolding hn_ctxt_def
+  apply(rule hnr_vcgI)
+  apply(simp add: nrest_more_simps ecost_le_zero) 
+  apply vcg
+  done
+
+
+end
+
+
+
 
 lemma hn_refineD:
   assumes "hn_refine \<Gamma> c \<Gamma>' R m"
